iris/WpKernelvecChain.v
@@ -43,6 +43,7 @@ Qed.
 
 Section Chain.
   Context `{!riscvGS Σ}.
+  Context (root_ppn : mword 44).
 
   (* Chain kernelvec's first two instructions: from the kernelvec entry (empty
      TLB + valid identity page table), run c.addi16sp sp,imm (fills the TLB) then
@@ -58,17 +59,17 @@ Section Chain.
     let spnew := add_vec vsp (sign_extend' 64 (caddi16sp_imm imm6)) in
     let a8 := sign_extend' 64 (subrange_vec_dec (add_vec spnew (sign_extend' 64 (zero_extend' 12 (concat_vec (mword_of_int 0 : mword 6) ('b"000"))))) (xlen - 0 - 1) 0) in
     let pa := zero_extend' 64 (add_vec_int a8 (0 * 8)) in
-    let tlbf := vec_update_dec tlbvec 5 (Some (pw_tlb_entry (mword_of_int 0))) in
+    let tlbf := vec_update_dec tlbvec 5 (Some (pw_tlb_entry root_ppn (mword_of_int 0))) in
     let mst1 := if b1 then add_vec_int mst0 1 else mst0 in
     m !! gpr_of_Z 2 = Some vsp ->
     m !! gpr_of_Z 1 = Some vra ->
     _get_Mstatus_SXL mstatus0 = 'b"10" ->
     _get_Satp64_Mode (Mk_Satp64 satp0) = ('b"1000" : mword 4) ->
-    autocast (T := mword) (satp_to_ppn (autocast (T := mword) satp0 : mword 64)) = (mword_of_int 0x80100 : mword 44) ->
+    autocast (T := mword) (satp_to_ppn (autocast (T := mword) satp0 : mword 64)) = root_ppn ->
     zero_extend' 16 (satp_to_asid (autocast (T := mword) satp0 : mword 64)) = (mword_of_int 0 : mword 16) ->
     vec_access_dec tlbvec 5 = None ->
     pma_allows_all pmar0 ->
-    matching_pma_region pmar0 (Physaddr (mword_of_int 0x80100010)) 8 = Some region_pte ->
+    matching_pma_region pmar0 (Physaddr (pte_paddr root_ppn)) 8 = Some region_pte ->
     (override_PMA (PMA_Region_attributes region_pte) PBMT_PMA).(PMA_supports_pte_read) = true ->
     matching_pma_region pmar0 (Physaddr (mword_of_int 0x800053e2)) 2 = Some region_f2 ->
     (override_PMA (PMA_Region_attributes region_f2) PBMT_PMA).(PMA_executable) = true ->
@@ -83,7 +84,7 @@ Section Chain.
       (uint (mword_of_int 0x800053e0 : mword 64)) (uint (to_bits 64 4)) = PMP_Match ->
     pmpRangeMatch (Z.mul (uint (zeros' 64 : mword 64)) 4)
       (Z.mul (uint (vec_access_dec pmpaddr00 0)) 4)
-      (uint (mword_of_int 0x80100010 : mword 64)) (uint (to_bits 64 8)) = PMP_Match ->
+      (uint (pte_paddr root_ppn : mword 64)) (uint (to_bits 64 8)) = PMP_Match ->
     pmpRangeMatch (Z.mul (uint (zeros' 64 : mword 64)) 4)
       (Z.mul (uint (vec_access_dec pmpaddr00 0)) 4)
       (uint (mword_of_int 0x800053e2 : mword 64)) (uint (to_bits 64 2)) = PMP_Match ->
@@ -94,7 +95,7 @@ Section Chain.
     eq_vec (_get_Pmpcfg_ent_R (vec_access_dec pmpcfg0 0)) ('b"1") = true ->
     eq_vec (_get_Pmpcfg_ent_W (vec_access_dec pmpcfg0 0)) ('b"1") = true ->
     is_aligned_paddr (Physaddr (mword_of_int 0x800053e0)) 4 = true ->
-    is_aligned_paddr (Physaddr (mword_of_int 0x80100010)) 8 = true ->
+    is_aligned_paddr (Physaddr (pte_paddr root_ppn)) 8 = true ->
     is_aligned_paddr (Physaddr (mword_of_int 0x800053e2)) 2 = true ->
     is_aligned_vaddr (Virtaddr a8) 8 = true ->
     is_aligned_paddr (Physaddr pa) 8 = true ->
@@ -126,7 +127,7 @@ Section Chain.
     tlb ↦ᵣ tlbvec -∗ menvcfg ↦ᵣ menvcfg0 -∗ mseccfg ↦ᵣ mseccfg0 -∗ mie ↦ᵣ mie_v -∗
     elp ↦ᵣ elp0 -∗ mcountinhibit ↦ᵣ mc -∗ minstretcfg ↦ᵣ mcfg -∗
     pmpcfg_n ↦ᵣ pmpcfg0 -∗ pmpaddr_n ↦ᵣ pmpaddr00 -∗ pma_regions ↦ᵣ pmar0 -∗ htif_tohost_base ↦ᵣ None -∗
-    ([∗ list] j ∈ seq 0 8, (pa_add (mword_of_int 0x80100010) j) ↦ₘ{dq} nth_byte pte_super j) -∗
+    ([∗ list] j ∈ seq 0 8, (pa_add (pte_paddr root_ppn) j) ↦ₘ{dq} nth_byte pte_super j) -∗
     ([∗ list] j ∈ seq 0 4, (pa_add (mword_of_int 0x800053e0) j) ↦ₘ{dq} nth_byte w1 j) -∗
     ([∗ list] j ∈ seq 0 2, (pa_add (mword_of_int 0x800053e2) j) ↦ₘ{dq} nth_byte w2 j) -∗
     ([∗ list] j ∈ seq 0 8, (pa_add pa j) ↦ₘ nth_byte vra j) -∗
@@ -139,7 +140,7 @@ Section Chain.
         tlb ↦ᵣ tlbf -∗ menvcfg ↦ᵣ menvcfg0 -∗ mseccfg ↦ᵣ mseccfg0 -∗ mie ↦ᵣ mie_v -∗
         elp ↦ᵣ elp0 -∗ mcountinhibit ↦ᵣ mc -∗ minstretcfg ↦ᵣ mcfg -∗
         pmpcfg_n ↦ᵣ pmpcfg0 -∗ pmpaddr_n ↦ᵣ pmpaddr00 -∗ pma_regions ↦ᵣ pmar0 -∗ htif_tohost_base ↦ᵣ None -∗
-        ([∗ list] j ∈ seq 0 8, (pa_add (mword_of_int 0x80100010) j) ↦ₘ{dq} nth_byte pte_super j) -∗
+        ([∗ list] j ∈ seq 0 8, (pa_add (pte_paddr root_ppn) j) ↦ₘ{dq} nth_byte pte_super j) -∗
         ([∗ list] j ∈ seq 0 4, (pa_add (mword_of_int 0x800053e0) j) ↦ₘ{dq} nth_byte w1 j) -∗
         ([∗ list] j ∈ seq 0 2, (pa_add (mword_of_int 0x800053e2) j) ↦ₘ{dq} nth_byte w2 j) -∗
         ([∗ list] j ∈ seq 0 8, (pa_add pa j) ↦ₘ nth_byte vra j) -∗
@@ -154,7 +155,7 @@ Section Chain.
     assert (HPC2 : add_vec_int (mword_of_int 0x800053e0 : mword 64) 2 = mword_of_int 0x800053e2)
       by (apply bv_eq; vm_compute; reflexivity).
     (* ---- instruction 1: c.addi16sp ---- *)
-    iApply (wp_pagewalk_caddi16sp w1 imm6 m vsp misa0 mdv0 mstatus0 menvcfg0 satp0 mie_v b1 npc0 mst0 mc mcfg
+    iApply (wp_pagewalk_caddi16sp root_ppn w1 imm6 m vsp misa0 mdv0 mstatus0 menvcfg0 satp0 mie_v b1 npc0 mst0 mc mcfg
               pmpcfg0 pmpaddr00 pmar0 mi0 elp0 tlbvec region_pte E Phi
               Hsp HSXL Hmode Hppn Hasid Hvec Hpmaall Hmatchp Hpte HPBMTE HA0 Hord0 Hr1 Hrpte HX0 HR0 Hal4 Halpte HisRVC1
               HmisaC HmisaS Hdec1 Hb1 Hmie_mdl HSIE Help
@@ -163,12 +164,12 @@ Section Chain.
     iIntros "Hpc Hfile Hmisa Hnpc Hmi Hmst Hpriv Hhs Hmdl Hms Hsatp Htlb Hmenv Hmie Help' Hmcinh Hmcfg Hpmpc Hpmpaddr Hpma Hhtif Hpbytes Hib1".
     rewrite !HPC2.
     (* ---- instruction 2: c.sdsp ra,0(sp) ---- *)
-    iApply (wp_pagewalk_csdsp w2 (mword_of_int 0) (mword_of_int 1)
+    iApply (wp_pagewalk_csdsp root_ppn w2 (mword_of_int 0) (mword_of_int 1)
               (<[gpr_of_Z 2 := regval_into_reg spnew]> m) (regval_into_reg spnew) vra misa0 mdv0 mstatus0 menvcfg0 mseccfg0 satp0 mie_v
               b1 vra (mword_of_int 0x800053e2) mst1 mc mcfg pmpcfg0 pmpaddr00 pmar0 b1 elp0 tlbf region_st region_f2 E Phi
               ltac:(vm_compute; discriminate)
               (lookup_insert _ _ _) ltac:(rewrite lookup_insert_ne; [ exact Hra | vm_compute; discriminate ])
-              HSXL Hmode Hasid (vec_access_update_5 tlbvec (pw_tlb_entry (mword_of_int 0)))
+              HSXL Hmode Hasid (vec_access_update_5 tlbvec (pw_tlb_entry root_ppn (mword_of_int 0)))
               Hmatchf2 Hexecf2 Hmatchst Hwrite Hpmm
               HA0 Hord0 Hr2 Hrst HX0 HW0 Hal2 Hal8 Hpal8 HisRVC2 HmisaC HmisaS HMPRV HMXR
               ltac:(intros s' Hcp Hsa Htl Hsx; apply Htr; assumption)
